separete test.v to myColoringSmallGraphs.v and myGraphs_Properties.v

vfa/myColoringSmallGraphs.v
@@ -1,9 +1,67 @@
 From VFA Require Import Color.
 From VFA Require Import Perm.
 From VFA Require Import myGraphs.
+From VFA Require Import Graphs_Properties.
 
 
 Open Scope positive.
+
+(* Monochromatic triplet in H with center. *)
+
+Definition center (g : graph) (o : node) : Prop :=
+  forall i, S.In i (nodes g) -> i <> o -> edge g i o.
+
+Definition H_center (o : node) : Prop :=
+  (gr_deg H o) = 6%nat.
+
+Compute (gr_deg H 1).
+
+Compute gr_show H.
+
+Lemma H_center_iff : forall o, center H o <-> o = 1.
+Proof.
+split; intro.
+-  unfold center in H. Print H.
+-  rewrite H. reflexivity.
+Qed.
+
+
+Check subset_nodes.
+
+Definition gr_deg_search (g : graph) (d : nat) : nodeset :=
+  subset_nodes (fun _ a => Nat.eqb (S.cardinal a) d) g.
+
+Compute S.elements (gr_deg_search H 0).
+
+Fixpoint gr_deg_sort (g : graph) (maxd : nat) : list (list node) :=
+  match maxd with
+  | 0%nat => [S.elements (gr_deg_search g 0)]
+  | S n => S.elements (gr_deg_search g maxd) :: gr_deg_sort g n
+  end.
+
+Compute gr_deg_sort H 6.
+
+
+Definition node_color (clr : coloring) (n : node) (c : S.elt) :=
+  M.find n clr = Some c.
+
+
+Definition monochrom (g : graph) (clr : coloring) (o l m n : node) :=
+  is_edge g o l /\ is_edge g o m /\ is_edge g o n /\ 
+   exists c, (node_color clr l c /\ node_color clr m c /\ node_color clr n c).
+
+
+
+Lemma H_monochrom_center : forall (plt : S.t) (clr : coloring) (o l m n : node),
+  coloring_ok plt H clr -> monochrom H clr o l m n -> H_center H o.
+
+
+
+Definition palette4: S.t := fold_right S.add S.empty [1; 2; 3; 4].
+
+Compute (M.elements (color palette H)).
+
+
 
 
 Search ( _  In  ).
